dev/lf/mutation-readme.md
@@ -1,0 +1,64 @@
+# Correspondence Between Coq Proof and Mutable WadlerFest DOT Paper
+
+## Abstract syntax
+
+In the paper, the abstract syntax is shown in Figure 1.
+
+In the proof, variables are represented using the inductive `avar` type, which can refer to a named or de Bruin indexed variable. The stack γ is represented using `stack`, which is a list of pairs of variables and values. The mutable store σ is represented using `store`, a map from addresses (locations) to variables. The type environment Γ is a list of pairs of variables and types `ctx`, and the store typing Σ is a list `store` of pairs of addresses and types.
+
+Types are represented using the datatype `typ`, terms using `trm`.
+
+## Reduction Rules
+
+In the paper, the reduction rules are shown in Figure 5.
+
+In the proof, the operational semantics is defined in the inductive relation `red`. 
+`red γ σ t γ' σ' t'` denotes the reduction step σ|γ|t ⟼  σ'|γ'|t'.
+
+## Type Rules
+
+The typing and subtyping rules are depicted in Figures 4 and 5 of the paper.
+
+In the proof, they are defined through mutual induction using the inductive definitions `ty_trm` and `subtyp`. A typing relation is characterized using two modes: 
+- `tymode`, which can be `ty_precise` or `ty_general` (precise or general typing), and
+- `submode`, which can be `sub_tight` or `sub_general` (tight or general subtyping).
+
+`ty_trm m₁ m₂ Γ Σ t T` corresponds to the typing relation Γ, Σ ⊢ t: T with typing and subtyping modes m₁ and m₂.
+
+Similarly, `subtyp m₁ m₂ Γ Σ T U` corresponds to the subtyping relation Γ, Σ ⊢ T <: U with modes m₁ and m₂.
+
+## Stack Correspondence and Well-Typedness
+
+A stack that corresponds to an environment, written in the paper as Γ, Σ ~ γ, is expressed using the inductive relation `wf_stack`: `wf_stack Γ Σ γ`.
+
+A well-typed store, denoted as Γ, Σ ⊢ σ, is expressed using the inductive relation `wt_store`: `wt_store Γ Σ γ`.
+
+## Type Safety Proof
+
+### Canonical Forms Lemma
+
+There are three canonical-forms lemma corresponding to Lemma 1, 2, and 3 in the paper, one for each type of values.
+
+1) `canonical_forms_1`
+  If Γ, Σ ⊢ x: ∀(x: T)U then γ(x)=λ(x: T').t for some T' and t such that 
+  - Γ, Σ ⊢ T <: T' and 
+  - (Γ, x: T), Σ ⊢ t: U.
+
+2) `canonical_forms_2`
+  If Γ, Σ ⊢ x: {a: T} then γ(x)=ν(x: S)d for some S, d, t such that
+  - Γ, Σ ⊢ d: S,
+  - {a = t} ∈ d,
+  - Γ, Σ ⊢ t: T.
+
+3) `canonical_forms_3`
+  If Γ, Σ ⊢ x: Ref T then γ(x)=l and σ(l)=y for some l, y such that
+  - Γ, Σ ⊢ l: Ref T and
+  - Γ, Σ ⊢ y: T.
+
+### Substitution
+
+The substitution principle (Lemma 2) in the proof is expressed in the Coq lemma `subst_rules`. It consists of the conjunction of four substatements, which reason about substitution in type rules, definition and multiple-definition typing judgements, and subtyping rules.
+
+### Soundness
+
+The main typesafety lemma (Proposition 1) is expressed in the `safety` lemma.
